cleanup definitions

IntroToCp/SimpleChoreographies.lean
@@ -1,192 +1,62 @@
-import Mathlib.Data.Set.Lattice
+import Mathlib.Order.Disjoint
+import Mathlib.Data.Finset.Basic
+import Mathlib.Data.Fintype.Basic
 import «IntroToCp».Relation
+import «IntroToCp».Name
 
-open Set
+variable {α : Type} [DecidableEq α] [fin : Fintype α]
 
 -- # Simple Choreographies
 
 -- ## Syntax
 
-structure PName where
-  name : String
-deriving BEq, DecidableEq
-
-#eval PName.mk "foo" == PName.mk "bar"
-
--- Coercion from String to PName
-instance : Coe String PName :=
-  ⟨PName.mk⟩
-
-instance : ToString PName where
-  toString := PName.name
-
-instance : Repr PName where
-  reprPrec p prec := p.name
-
-#eval ("x" : PName)
-
-def disjoint (a : Set α) (b : Set α) : Prop := ∀ x y, x ∈ a → y ∈ b → x ≠ y
-
-def s₁ : Set Nat := {1, 2, 3}
-def s₂ : Set Nat := {4, 5, 6}
-
-example : disjoint s₁ s₂ := by
-  simp [disjoint]
-  intro x' y' h1 h2
-  cases h1 with
-  | inl h1 => cases h2 with
-    | inl h2 => simp [h1, h2]
-    | inr h2 => cases h2 with
-      | inl h2 => simp [h1, h2]
-      | inr h2 => rw [mem_singleton_iff] at h2
-                  simp [h1, h2]
-  | inr h1 => cases h2 with
-    | inl h2 => cases h1 with
-      | inl h1 => simp [h1, h2]
-      | inr h1 => rw [mem_singleton_iff] at h1
-                  simp [h1, h2]
-    | inr h2 => cases h1 with
-      | inl h1 => cases h2 with
-        | inl h2 => simp [h1, h2]
-        | inr h2 => rw [mem_singleton_iff] at h2
-                    simp [h1, h2]
-      | inr h1 => cases h2 with
-        | inl h2 => rw [mem_singleton_iff] at h1
-                    simp [h1, h2]
-        | inr h2 => rw [mem_singleton_iff] at h1
-                    rw [mem_singleton_iff] at h2
-                    simp [h1, h2]
-
-inductive SimpleChor : Type where
-  | done : SimpleChor
-  -- TODO: do I need p ≠ q?
-  | comm (p : PName) (q : PName) (C : SimpleChor) : SimpleChor
-deriving Repr
+inductive SimpleChor (α : Type) where
+  | done : SimpleChor α
+  | comm (p : α) (q : α) (C : SimpleChor α) : SimpleChor α
+deriving Repr, DecidableEq
 
 -- terminated choreography
-def 𝕆 := SimpleChor.done
+def SimpleChor.𝕆 : SimpleChor α := SimpleChor.done
 
 notation:10 p " ~> " q " ; " C => SimpleChor.comm p q C
 
--- example 2.2
-#eval "buyer" ~> "seller" ; "seller" ~> "buyer" ; 𝕆
+-- Example 2.2
+#eval Name.buyer ~> Name.seller ; Name.seller ~> Name.buyer ; SimpleChor.done
 
 -- Exercise 2.1
-def ringProtocol := "Alice" ~> "Bob" ; "Bob" ~> "Charlie" ; "Charlie" ~> "Alice" ; 𝕆
+def ringProtocol := Name.alice ~> Name.bob ; Name.bob ~> Name.charlie ; Name.charlie ~> Name.alice ; SimpleChor.done
 
 -- Exercise 2.2
-def scatterProtocol := "Alice" ~> "Bob" ; "Alice" ~> "Charlie" ; 𝕆
+def scatterProtocol := Name.alice ~> Name.bob ; Name.alice ~> Name.charlie ; SimpleChor.done
 
-def pn (s : α × α) : Set α := {s.fst, s.snd}
+-- Semantics
 
-#check pn (("Alice", "Bob"))
+def pn (s : α × α) : Finset α := {s.fst, s.snd}
 
-inductive Transition : SimpleChor → (PName × PName) → SimpleChor → Prop where
-  -- p ~> q ; C → ⟨ p, q ⟩ → C
-  | comm : ∀ {p q C}, Transition (p ~> q ; C) (p, q) C
-  | delay : Transition C μ C' → disjoint {p, q} (pn μ) → Transition (p ~> q; C) μ (p ~> q; C')
+inductive SimpleChor.Step : SimpleChor α → (α × α) → SimpleChor α → Prop where
+  | comm : ∀ {p q : α} {C : SimpleChor α}, Step (p ~> q ; C) (p, q) C
+  | delay : ∀ {C C': SimpleChor α} {μ : (α × α)}, Step C μ C' → Disjoint {p, q} (pn μ) → Step (p ~> q ; C) μ (p ~> q ; C')
 
 -- Example 2.3
-example : Transition ("buyer" ~> "seller" ; "seller" ~> "buyer" ; 𝕆) ("buyer", "seller") ("seller" ~> "buyer" ; 𝕆) := by
-  apply Transition.comm
+example : SimpleChor.Step
+  (Name.buyer ~> Name.seller ; Name.seller ~> Name.buyer ; SimpleChor.done)
+  (Name.buyer, Name.seller)
+  (Name.seller ~> Name.buyer ; SimpleChor.done) := by apply SimpleChor.Step.comm
 
--- Exercise 2.3
-example : Transition ringProtocol ("Alice", "Bob") ("Bob" ~> "Charlie" ; "Charlie" ~> "Alice" ; 𝕆) := by
-  apply Transition.comm
-example : Transition ("Bob" ~> "Charlie" ; "Charlie" ~> "Alice" ; 𝕆) ("Bob", "Charlie") ("Charlie" ~> "Alice" ; 𝕆) := by
-  apply Transition.comm
-example : Transition ("Charlie" ~> "Alice" ; 𝕆) ("Charlie", "Alice") 𝕆 := by
-  apply Transition.comm
+inductive SimpleChor.MultiStep : SimpleChor α → List (α × α) → SimpleChor α → Prop where
+  | rfl : ∀ (C: SimpleChor α), MultiStep C [] C
+  | step : ∀ (C: SimpleChor α) (μ : (α × α)) (C' : SimpleChor α) (μ' : List (α × α)) (C'' : SimpleChor α),
+      Step C μ C' → MultiStep C' μ' C'' → MultiStep C (μ :: μ') C''
 
-example : Transition scatterProtocol ("Alice", "Bob") ("Alice" ~> "Charlie" ; 𝕆) := by
-  apply Transition.comm
-example : Transition ("Alice" ~> "Charlie" ; 𝕆) ("Alice", "Charlie") 𝕆 := by
-  apply Transition.comm
-
--- Example 2.4
-example : Transition ("buyer₁" ~> "seller₁" ; "buyer₂" ~> "seller₂" ; 𝕆) ("buyer₂", "seller₂") ("buyer₁" ~> "seller₁" ; 𝕆) := by
-  apply Transition.delay
-  . apply Transition.comm
-  . simp [pn, disjoint]
-    intro x y hx hy
-    apply hx.elim <;> intro hx
-    all_goals (apply hy.elim)
-    all_goals intro c hc
-    all_goals (simp [*] at * ; contradiction)
-
--- Example 2.5
-example := "p₁" ~> "q₁" ; "p₂" ~> "q₂" ; "p₃" ~> "q₃" ; 𝕆
-example : Transition
-            ("p₁" ~> "q₁" ; "p₂" ~> "q₂" ; "p₃" ~> "q₃" ; 𝕆)
-            ("p₃", "q₃")
-            ("p₁" ~> "q₁" ; "p₂" ~> "q₂" ; 𝕆) := by
-            apply Transition.delay
-            . apply Transition.delay
-              . apply Transition.comm
-              . simp [disjoint]
-                intro p q hp hq
-                intro c
-                cases hp with
-                | inl hp =>
-                  cases hq with
-                  | inl hq =>
-                    simp at hq
-                    simp [hp, hq] at c
-                    contradiction
-                  | inr hq =>
-                    simp at hq
-                    simp [hp, hq] at c
-                    contradiction
-                | inr hp =>
-                  cases hq with
-                  | inl hq =>
-                    simp at hq
-                    simp [hp, hq] at c
-                    contradiction
-                  | inr hq =>
-                    simp at hq
-                    simp [hp, hq] at c
-                    contradiction
-            . simp [disjoint]
-              intro p q hp hq
-              intro c
-              cases hp with
-              | inl hp =>
-                cases hq with
-                | inl hq =>
-                  simp at hq
-                  simp [hp, hq] at c
-                  contradiction
-                | inr hq =>
-                  simp at hq
-                  simp [hp, hq] at c
-                  contradiction
-              | inr hp =>
-                cases hq with
-                | inl hq =>
-                  simp at hq
-                  simp [hp, hq] at c
-                  contradiction
-                | inr hq =>
-                  simp at hq
-                  simp [hp, hq] at c
-                  contradiction
-
-
--- Exercise 6: theee communications can be done in any order
-
--- ## 2.3 Conventions, Notation, and Terminology for Labelled Transition Systems
-
-inductive MultiTransition : SimpleChor → List (PName × PName) → SimpleChor → Prop where
-  | rfl : ∀ c, MultiTransition c [] c
-  | step : ∀ c μ c' μ' c'',
-      Transition c μ c' → MultiTransition c' μ' c'' → MultiTransition c (μ::μ') c''
-
-example : MultiTransition ("p₁" ~> "q₁" ; "p₂" ~> "q₂" ; "p₃" ~> "q₃" ; 𝕆) [("p₁", "q₁"), ("p₂", "q₂"), ("p₃", "q₃")] 𝕆 := by
-  apply MultiTransition.step _ _ ("p₂" ~> "q₂" ; "p₃" ~> "q₃" ; 𝕆)
-  constructor
-  apply MultiTransition.step _ _ ("p₃" ~> "q₃" ; 𝕆)
-  constructor
-  apply MultiTransition.step _ _ 𝕆
-  constructor
-  apply MultiTransition.rfl
+example : SimpleChor.MultiStep
+  (Name.p₁ ~> Name.q₁ ; Name.p₂ ~> Name.q₂ ; Name.p₃ ~> Name.q₃ ; SimpleChor.𝕆)
+  [(Name.p₁, Name.q₁), (Name.p₂, Name.q₂), (Name.p₃, Name.q₃)]
+  SimpleChor.𝕆
+:= by
+  apply SimpleChor.MultiStep.step _ _ (Name.p₂ ~> Name.q₂ ; Name.p₃ ~> Name.q₃ ; SimpleChor.𝕆) _ _
+  apply SimpleChor.Step.comm
+  apply SimpleChor.MultiStep.step _ _ (Name.p₃ ~> Name.q₃ ; SimpleChor.𝕆) _ _
+  apply SimpleChor.Step.comm
+  apply SimpleChor.MultiStep.step _ _ (SimpleChor.𝕆) _ _
+  apply SimpleChor.Step.comm
+  apply SimpleChor.MultiStep.rfl
