IntroToCp/Name.lean
@@ -1,0 +1,23 @@
+import Mathlib.Data.Fintype.Basic
+
+inductive Name where
+| alice : Name
+| bob : Name
+| charlie : Name
+| buyer : Name
+| seller : Name
+| p₁ : Name
+| q₁ : Name
+| p₂ : Name
+| q₂ : Name
+| p₃ : Name
+| q₃ : Name
+
+deriving Repr, DecidableEq
+
+instance : Fintype Name where
+  elems := {Name.alice, Name.bob, Name.charlie, Name.buyer, Name.seller, Name.p₁, Name.q₁, Name.p₂, Name.q₂, Name.p₃, Name.q₃}
+  complete := by
+    intro n
+    simp
+    cases n <;> simp
